Add exploitation of data races

theories/simplang/examples/data_races.v
@@ -1,4 +1,4 @@
-From simuliris.simplang Require Import lang notation tactics class_instances heap_bij.
+From simuliris.simplang Require Import lang notation tactics class_instances proofmode heap_bij_races.
 From iris Require Import bi.bi.
 Import bi.
 From iris.proofmode Require Import tactics.
@@ -7,7 +7,12 @@ From simuliris.simulation Require Import slsls lifting.
 (** * Examples for exploiting UB of data-races. *)
 
 Section data_race.
-  Context `{sbijG Σ}.
+  Context `{nabijG Σ}.
+
+  (*
+    problem of establishing disjointness:
+    option 1: add comparsion in target (and make op sem for that realistic)
+*)
 
   Definition remove_store_and_load_opt :=
     (λ: "a", let: "l1" := Fst "a" in
@@ -27,9 +32,9 @@ Section data_race.
     )%E.
 
   Lemma remove_store_and_load_sim π:
-    ⊢ sim_ectx (const val_rel) π remove_store_and_load_opt remove_store_and_load val_rel.
+    ⊢ sim_ectx (weak_val_rel) π remove_store_and_load_opt remove_store_and_load val_rel.
   Proof.
-    iIntros (v_t v_s) "Hrel". sim_pures.
+    iIntros (v_t v_s) "[Hc Hrel]". sim_pures.
 
     source_bind (Fst v_s).
     iApply source_red_irred_unless; first done.
@@ -37,8 +42,19 @@ Section data_race.
     iPoseProof (val_rel_pair_source with "Hrel") as (v_t1 v_t2) "(-> & #Hrel1 & Hrel2')".
     sim_pures.
     sim_pures.
+    source_bind (! _)%E.
+    iApply source_red_irred_unless; first done.
+    iIntros ((l_s2 & ->)).
+    iPoseProof (val_rel_loc_source with "Hrel2'") as (l_t2 ->) "#Hrel2".
+    sim_pures. simpl. rewrite -!source_red_base. do 2 iModIntro.
 
+    sim_bind (_) (! _)%E.
   Abort.
+    (* iApply (sim_bij_exploit_load with "Hrel2 Hc"); [intros; apply: no_forks_refl|done|]. *)
+    (* iIntros (q v_t v_s) "Hl_t2 Hl_s2 Hv Hc". iApply sim_expr_base. *)
+    (* source_load. target_load. sim_pures. *)
+
+  (* Abort. *)
 
   Definition reg_promote_loop_opt f :=
     (λ: "a",
@@ -91,51 +107,161 @@ Section data_race.
   Definition hoist_load_opt :=
     (λ: "a",
      let: "n" := Fst "a" in
-     let: "m" := Fst (Snd "a") in
-     let: "x" := Snd (Snd "a") in
-     let: "refi" := ref #0 in
+     let: "m" := Snd "a" in
      if: "n" < #1 then
        #0
      else
        let: "mval" := !"m" in
-       while: ! "refi" < "n" do
-         "x" <- "mval";;
-         "refi" <- !"refi" + #1
+       let: "r" := ref "mval" in
+       let: "i" := ref #1 in
+       while: ! "i" < "n" do
+         "r" <- !"r" + "mval";;
+         (* Call ##f "x";; *)
+         "i" <- !"i" + #1
        od;;
-       #0
+       Free "i";;
+       let: "res" := !"r" in
+       Free "r";;
+       "res"
     )%E.
 
   Definition hoist_load :=
     (λ: "a",
      let: "n" := Fst "a" in
-     let: "m" := Fst (Snd "a") in
-     let: "x" := Snd (Snd "a") in
-     let: "refi" := ref #0 in
-     while: ! "refi" < "n" do
-       "x" <- !"m";;
-       "refi" <- !"refi" + #1
+     let: "m" := Snd "a" in
+     let: "r" := ref #0  in
+     let: "i" := ref #0  in
+     while: ! "i" < "n" do
+       "r" <- !"r" + !"m";;
+       (* Call ##f "x";; *)
+       "i" <- !"i" + #1
      od;;
-       #0
+     Free "i";;
+     let: "res" := !"r" in
+     Free "r";;
+     "res"
     )%E.
 
   Lemma hoist_load_sim π:
-    ⊢ sim_ectx (const val_rel) π hoist_load_opt hoist_load val_rel.
+    ⊢ sim_ectx (weak_val_rel) π hoist_load_opt hoist_load val_rel.
   Proof.
-    iIntros (v_t v_s) "Hrel". sim_pures.
+    iIntros (v_t v_s) "[Hc Hrel]". sim_pures.
 
     source_bind (Fst v_s).
     iApply source_red_irred_unless; first done.
     iIntros ((v_s1 & v_s2' & ->)).
     sim_pures.
 
-    source_bind (Fst v_s2').
-    iApply source_red_irred_unless; first done.
-    iIntros ((v_s2 & v_s3 & ->)).
+    iPoseProof (val_rel_pair_source with "Hrel") as (v_t1 v_t2) "(-> & #Hrel1 & #Hrel2)".
     sim_pures.
+    source_alloc lr_s as "Hlr_s" "Hfr_s". sim_pures.
+    source_alloc li_s as "Hli_s" "Hfi_s". sim_pures.
+    source_while. source_load.
+    source_bind (_ < _)%E. iApply source_red_irred_unless; first done.
+    iIntros ([[??] [??]]); simplify_eq.
+    iDestruct (val_rel_litint_source with "Hrel1") as %->. sim_pures. sim_pures.
+    case_bool_decide; [rewrite bool_decide_false;[|lia]|rewrite bool_decide_true;[|lia]]; sim_pures.
+    - source_free. sim_pures. source_load. sim_pures. source_free. sim_pures. by sim_val.
+    - source_bind (! _)%E. iApply source_red_irred_unless; first done.
+      iIntros ([l_s ?]); simplify_eq.
+      iDestruct (val_rel_loc_source with "Hrel2") as (l_t ->) "Hbij".
+      do 2 iApply source_red_base. do 2 iModIntro.
+      iApply (sim_bij_exploit_load with "Hbij Hc"); [|done|]. {
+        intros. reach_or_stuck_fill (! _)%E => /=.
+        apply: reach_or_stuck_refl. apply: post_in_ectx_intro. naive_solver.
+      }
+      iIntros (q v_t v_s) "Hl_t Hl_s #Hv Hc".
+      iDestruct (heap_mapsto_ne with "Hlr_s Hli_s") as %Hne1.
+      iDestruct (heap_mapsto_ne with "Hlr_s Hl_s") as %Hne2.
+      iDestruct (heap_mapsto_ne with "Hli_s Hl_s") as %Hne3.
+      source_load. sim_pures. source_load. sim_pures.
+      source_bind (_ + _)%E. iApply source_red_irred_unless; first done.
+      iIntros ([[??] [m ?]]); simplify_eq.
+      iDestruct (val_rel_litint_source with "Hv") as %->. sim_pures. rewrite Z.add_0_l.
+      source_store. source_load. source_store. sim_pures.
 
-    iPoseProof (val_rel_pair_source with "Hrel") as (v_t1 v_t2') "(-> & #Hrel1 & Hrel2')".
-    iPoseProof (val_rel_pair_source with "Hrel2'") as (v_t2 v_t3) "(-> & #Hrel2 & Hrel3)".
-    sim_pures.
+      target_load. target_alloc lr_t as "Hlr_t" "Hfr_t". target_alloc li_t as "Hli_t" "Hfi_t".
+      sim_pures.
+      iApply (sim_bij_insert with "Hfi_t Hfi_s Hli_t Hli_s []"); [done|]. iIntros "#Hbiji".
+      iApply (sim_bij_insert with "Hfr_t Hfr_s Hlr_t Hlr_s []"); [done|]. iIntros "#Hbijr".
+      sim_bind (While _ _) (While _ _).
+      iApply (sim_while_while _ _ _ _ _ _ (
+         l_t ↦t{#q} #m ∗ l_s ↦s{#q} #m ∗ na_locs π (<[l_s:=(l_t, NaRead q)]> ∅))%I with "[-]").
+      { eauto with iFrame. }
+      iIntros "!> (Hl_t&Hl_s&Hc)".
+      sim_bind (! _)%E (! _)%E.
+      iApply (sim_bij_load_na with "Hbiji Hc"); [by simplify_map_eq|].
+      iIntros (??) "Hv' Hc". sim_val.
+      source_bind (_ < _)%E. iApply source_red_irred_unless; first done.
+      iIntros ([[??] [??]]); simplify_eq.
+      iDestruct (val_rel_litint_source with "Hv'") as %->. sim_pures. sim_pures.
+      case_bool_decide; sim_pures.
+      + source_load. sim_pures.
+        sim_bind (! _)%E (! _)%E.
+        iApply (sim_bij_load_na with "Hbijr Hc"); [by simplify_map_eq|].
+        iIntros (??) "Hv'' Hc". sim_val.
+        source_bind (_ + _)%E. iApply source_red_irred_unless; first done.
+        iIntros ([[??] [??]]); simplify_eq.
+        iDestruct (val_rel_litint_source with "Hv''") as %->. sim_pures. sim_pures.
+        sim_bind (_ <- _)%E (_ <- _)%E.
+        iApply (sim_bij_store_na with "Hbijr Hc"); [by simplify_map_eq| done |].
+        iIntros "Hc". sim_val. sim_pures.
 
-  Abort.
+        sim_bind (! _)%E (! _)%E.
+        iApply (sim_bij_load_na with "Hbiji Hc"); [by simplify_map_eq|].
+        iIntros (??) "Hv''' Hc". sim_val.
+        source_bind (_ + _)%E. iApply source_red_irred_unless; first done.
+        iIntros ([[??] [??]]); simplify_eq.
+        iDestruct (val_rel_litint_source with "Hv'''") as %->. sim_pures. sim_pures.
+        sim_bind (_ <- _)%E (_ <- _)%E.
+        iApply (sim_bij_store_na with "Hbiji Hc"); [by simplify_map_eq| done |].
+        iIntros "Hc". sim_val. sim_pures.
+
+        iApply sim_expr_base. iRight. by iFrame.
+      + iApply sim_expr_base. iLeft. iApply lift_post_val.
+        sim_pures.
+        sim_bind (FreeN _ _)%E (FreeN _ _)%E.
+        iApply (sim_bij_free with "Hbiji Hc"). {
+          move => i ?. rewrite lookup_insert_ne //.
+          destruct (decide (i = 0%Z)); [subst |lia]. by rewrite loc_add_0.
+        }
+        iIntros "Hc". sim_val. sim_pures.
+        sim_bind (! _)%E (! _)%E.
+        iApply (sim_bij_load_na with "Hbijr Hc"); [by simplify_map_eq|].
+        iIntros (??) "Hv'' Hc". sim_val. sim_pures.
+        sim_bind (FreeN _ _)%E (FreeN _ _)%E.
+        iApply (sim_bij_free with "Hbijr Hc"). {
+          move => i ?. rewrite lookup_insert_ne //.
+          destruct (decide (i = 0%Z)); [subst |lia]. by rewrite loc_add_0.
+        }
+        iIntros "Hc". sim_val. sim_pures. by sim_val.
+  Qed.
+
+  (* TODO: try also other direction (or maybe another example that adds loads and that makes more sense) *)
+
+  Definition register_pressure_opt :=
+    (λ: "a",
+     let: "z" := !"a" + #1 in
+     "z" + !"a"
+    )%E.
+
+  Definition register_pressure_load :=
+    (λ: "a",
+     let: "y" := !"a" in
+     let: "z" := "y" + #1 in
+     "z" + "y"
+    )%E.
+
+
+  (* TODO: go over memory model papers (promising semantics paper)
+
+   prove some reorderings:
+   - reordering reads
+   - reordering writes to different locations
+   - compact two reads
+   - ...
+
+   TODO: try to find something about Concurrent CompCert, what is used by VST
+*)
+
 End data_race.
