theories/simplang/heapbij.v
@@ -1,0 +1,567 @@
+From iris.proofmode Require Import tactics.
+From iris.bi.lib Require Import fractional .
+From iris.base_logic.lib Require Import ghost_map.
+From simuliris.base_logic Require Export gen_sim_heap gen_sim_prog.
+From simuliris.simulation Require Import slsls lifting.
+From iris.algebra.lib Require Import gset_bij.
+From iris.base_logic.lib Require Import gset_bij.
+From simuliris.simplang Require Export class_instances primitive_laws.
+
+From iris.prelude Require Import options.
+
+Lemma take_lookup_Some {A} n k (l : list A) x:
+  take n l !! k = Some x ↔ l !! k = Some x ∧ k < n.
+Proof.
+  split.
+  - destruct (decide (k < n)).
+    + rewrite lookup_take; naive_solver.
+    + rewrite lookup_take_ge //. lia.
+  - move => [??]. by rewrite lookup_take.
+Qed.
+
+
+Class heapbijG (Σ : gFunctors) := HeapBijG {
+  heapbijG_sheapG :> sheapGS Σ;
+  heapbijG_bijG :> gset_bijG Σ block block;
+  heapbijG_bij_name : gname;
+}.
+
+Section definitions.
+  Context `{heapbijG Σ}.
+
+  Definition heap_bij_auth (L : gset (block * block)) :=
+    gset_bij_own_auth heapbijG_bij_name (DfracOwn 1) L.
+  Definition heap_bij_elem (l_t : block) (l_s : block) :=
+    gset_bij_own_elem heapbijG_bij_name l_t l_s.
+End definitions.
+
+Notation "b_t '⇔h' b_s" := (heap_bij_elem b_t b_s) (at level 30) : bi_scope.
+Definition loc_rel `{heapbijG Σ} l_t l_s : iProp Σ := loc_chunk l_t ⇔h loc_chunk l_s ∗ ⌜loc_idx l_t = loc_idx l_s⌝.
+Notation "l_t '↔h' l_s" := (loc_rel l_t l_s) (at level 30) : bi_scope.
+
+Section laws.
+  Context `{heapbijG Σ}.
+  Implicit Types (b_t b_s : block) (l_t l_s : loc).
+
+  Global Instance heap_bij_elem_persistent b_t b_s :
+    Persistent (b_t ⇔h b_s).
+  Proof. apply _. Qed.
+  Global Instance heap_bij_elem_loc_persistent l_t l_s :
+    Persistent (l_t ↔h l_s).
+  Proof. apply _. Qed.
+
+  Lemma heap_bij_agree b_t1 b_t2 b_s1 b_s2 :
+    b_t1 ⇔h b_s1 -∗ b_t2 ⇔h b_s2 -∗ ⌜b_t1 = b_t2 ↔ b_s1 = b_s2⌝.
+  Proof.
+    iIntros "H1 H2". iApply (gset_bij_own_elem_agree with "H1 H2").
+  Qed.
+  Lemma heap_bij_loc_agree l_t1 l_t2 l_s1 l_s2 :
+    l_t1 ↔h l_s1 -∗ l_t2 ↔h l_s2 -∗ ⌜l_t1 = l_t2 ↔ l_s1 = l_s2⌝.
+  Proof.
+    iIntros "[H1 %Heq1] [H3 %Heq2]".
+    iPoseProof (heap_bij_agree with "H1 H3") as "%Ha". iPureIntro.
+    destruct l_t1, l_t2, l_s1, l_s2; cbn in *; subst. naive_solver.
+  Qed.
+
+  Lemma heap_bij_func b_t b_s1 b_s2 :
+    b_t ⇔h b_s1 -∗ b_t ⇔h b_s2 -∗ ⌜b_s1 = b_s2⌝.
+  Proof.
+    iIntros "H1 H2". iPoseProof (heap_bij_agree with "H1 H2") as "<-"; done.
+  Qed.
+  Lemma heap_bij_loc_func l_t l_s1 l_s2 :
+    l_t ↔h l_s1 -∗ l_t ↔h l_s2 -∗ ⌜l_s1 = l_s2⌝.
+  Proof.
+    iIntros "H1 H2". iPoseProof (heap_bij_loc_agree with "H1 H2") as "<-"; done.
+  Qed.
+
+  Lemma heap_bij_inj b_s b_t1 b_t2 :
+    b_t1 ⇔h b_s -∗ b_t2 ⇔h b_s -∗ ⌜b_t1 = b_t2⌝.
+  Proof.
+    iIntros "H1 H2". iPoseProof (heap_bij_agree with "H1 H2") as "->"; done.
+  Qed.
+  Lemma heap_bij_loc_inj l_s l_t1 l_t2 :
+    l_t1 ↔h l_s -∗ l_t2 ↔h l_s -∗ ⌜l_t1 = l_t2⌝.
+  Proof.
+    iIntros "H1 H2". iPoseProof (heap_bij_loc_agree with "H1 H2") as "->"; done.
+  Qed.
+
+  Lemma heap_bij_loc_shift l_t l_s i : l_t ↔h l_s -∗ (l_t +ₗ i) ↔h (l_s +ₗ i).
+  Proof.
+    iIntros "[Hi %Hj]". iSplitL "Hi"; first done. iPureIntro.
+    destruct l_t, l_s; cbn in *; lia.
+  Qed.
+End laws.
+
+(** ** Default value relation *)
+Section val_rel.
+  Context `{heapbijG Σ}.
+  Fixpoint val_rel (v_t v_s : val) {struct v_s} : iProp Σ :=
+    match v_t, v_s with
+    | LitV (LitLoc l_t), LitV (LitLoc l_s) =>
+        l_t ↔h l_s
+    | LitV l_t, LitV l_s =>
+        ⌜l_t = l_s⌝
+    | PairV v1_t v2_t, PairV v1_s v2_s =>
+        val_rel v1_t v1_s ∧ val_rel v2_t v2_s
+    | InjLV v_t, InjLV v_s =>
+        val_rel v_t v_s
+    | InjRV v_t, InjRV v_s =>
+        val_rel v_t v_s
+    | _,_ => False
+    end.
+  Global Instance val_rel_pers v_t v_s : Persistent (val_rel v_t v_s).
+  Proof.
+    induction v_s as [[] | | | ] in v_t |-*; destruct v_t as [ [] | | | ]; apply _.
+  Qed.
+
+  Lemma val_rel_pair_source v_t v_s1 v_s2 :
+    val_rel v_t (v_s1, v_s2) -∗
+    ∃ v_t1 v_t2, ⌜v_t = PairV v_t1 v_t2⌝ ∗
+      val_rel v_t1 v_s1 ∗
+      val_rel v_t2 v_s2.
+  Proof.
+    simpl. iIntros "H". destruct v_t as [[] | v_t1 v_t2 | |]; simpl; try done.
+    iExists v_t1, v_t2. iDestruct "H" as "[#H1 #H2]". eauto.
+  Qed.
+  Lemma val_rel_injl_source v_t v_s :
+    val_rel v_t (InjLV v_s) -∗ ∃ v_t', ⌜v_t = InjLV v_t'⌝ ∗ val_rel v_t' v_s.
+  Proof. simpl. destruct v_t as [[] | | |]; (try by iIntros "%Hp"); eauto. Qed.
+  Lemma val_rel_injr_source v_t v_s :
+    val_rel v_t (InjRV v_s) -∗ ∃ v_t', ⌜v_t = InjRV v_t'⌝ ∗ val_rel v_t' v_s.
+  Proof. simpl. destruct v_t as [[] | | |]; (try by iIntros "%Hp"); eauto. Qed.
+
+
+  Lemma val_rel_litfn_source v_t fn_s :
+    val_rel v_t (LitV $ LitFn $ fn_s) -∗ ⌜v_t = LitV $ LitFn $ fn_s⌝.
+  Proof. simpl. destruct v_t as [[] | v_t1 v_t2 | |]; iIntros "%Hp"; inversion Hp; subst; done. Qed.
+  Lemma val_rel_litint_source v_t n :
+    val_rel v_t (LitV $ LitInt n) -∗ ⌜v_t = LitV $ LitInt $ n⌝.
+  Proof. simpl. destruct v_t as [[] | v_t1 v_t2 | |]; iIntros "%Hp"; inversion Hp; subst; done. Qed.
+  Lemma val_rel_litbool_source v_t b:
+    val_rel v_t (LitV $ LitBool b) -∗ ⌜v_t = LitV $ LitBool b⌝.
+  Proof. simpl. destruct v_t as [[] | v_t1 v_t2 | |]; iIntros "%Hp"; inversion Hp; subst; done. Qed.
+  Lemma val_rel_litunit_source v_t :
+    val_rel v_t (LitV $ LitUnit) -∗ ⌜v_t = LitV $ LitUnit⌝.
+  Proof. simpl. destruct v_t as [[] | v_t1 v_t2 | |]; iIntros "%Hp"; inversion Hp; subst; done. Qed.
+  Lemma val_rel_litpoison_source v_t :
+    val_rel v_t (LitV $ LitPoison) -∗ ⌜v_t = LitV $ LitPoison⌝.
+  Proof. simpl. destruct v_t as [[] | v_t1 v_t2 | |]; iIntros "%Hp"; inversion Hp; subst; done. Qed.
+  Lemma val_rel_loc_source v_t l_s :
+    val_rel v_t (LitV $ LitLoc l_s) -∗
+    ∃ l_t, ⌜v_t = LitV $ LitLoc l_t⌝ ∗ l_t ↔h l_s.
+  Proof.
+    destruct v_t as [[ | | | | l_t | ] | | | ]; simpl;
+        first [iIntros "%Ht"; congruence | iIntros "#Ht"; eauto].
+  Qed.
+
+  Lemma val_rel_pair_target v_s v_t1 v_t2 :
+    val_rel (v_t1, v_t2) v_s -∗
+    ∃ v_s1 v_s2, ⌜v_s = PairV v_s1 v_s2⌝ ∗
+      val_rel v_t1 v_s1 ∗
+      val_rel v_t2 v_s2.
+  Proof.
+    simpl. iIntros "H". destruct v_s as [[] | v_s1 v_s2 | |]; simpl; try done.
+    iExists v_s1, v_s2. iDestruct "H" as "[#H1 #H2]". eauto.
+  Qed.
+  Lemma val_rel_injl_target v_t v_s :
+    val_rel (InjLV v_t) v_s -∗ ∃ v_s', ⌜v_s = InjLV v_s'⌝ ∗ val_rel v_t v_s'.
+  Proof. simpl. destruct v_s as [[] | | |]; (try by iIntros "%Hp"); eauto. Qed.
+  Lemma val_rel_injr_target v_t v_s :
+    val_rel (InjRV v_t) v_s -∗ ∃ v_s', ⌜v_s = InjRV v_s'⌝ ∗ val_rel v_t v_s'.
+  Proof. simpl. destruct v_s as [[] | | |]; (try by iIntros "%Hp"); eauto. Qed.
+  Lemma val_rel_litfn_target v_s fn_t :
+    val_rel (LitV $ LitFn $ fn_t) v_s -∗ ⌜v_s = LitV $ LitFn $ fn_t⌝.
+  Proof. simpl. destruct v_s as [[] | v_s1 v_s2 | |]; iIntros "%Hp"; inversion Hp; subst; done. Qed.
+  Lemma val_rel_litint_target v_s n :
+    val_rel (LitV $ LitInt n) v_s -∗ ⌜v_s = LitV $ LitInt $ n⌝.
+  Proof. simpl. destruct v_s as [[] | | |]; iIntros "%Hp"; inversion Hp; subst; done. Qed.
+  Lemma val_rel_litbool_target v_s b:
+    val_rel (LitV $ LitBool b) v_s -∗ ⌜v_s = LitV $ LitBool b⌝.
+  Proof. simpl. destruct v_s as [[] | | |]; iIntros "%Hp"; inversion Hp; subst; done. Qed.
+  Lemma val_rel_litunit_target v_s :
+    val_rel (LitV $ LitUnit) v_s -∗ ⌜v_s = LitV $ LitUnit⌝.
+  Proof. simpl. destruct v_s as [[] | | |]; iIntros "%Hp"; inversion Hp; subst; done. Qed.
+  Lemma val_rel_litpoison_target v_s :
+    val_rel (LitV $ LitPoison) v_s -∗ ⌜v_s = LitV $ LitPoison⌝.
+  Proof. simpl. destruct v_s as [[] | | |]; iIntros "%Hp"; inversion Hp; subst; done. Qed.
+  Lemma val_rel_loc_target v_s l_t :
+    val_rel (LitV $ LitLoc l_t) v_s -∗
+    ∃ l_s, ⌜v_s = LitV $ LitLoc l_s⌝ ∗ l_t ↔h l_s.
+  Proof.
+    destruct v_s as [[ | | | | l_s | ] | | | ]; simpl;
+        first [iIntros "%Hs"; congruence | iIntros "#Hs"; eauto].
+  Qed.
+End val_rel.
+Tactic Notation "val_discr_source" constr(H) :=
+  first [iPoseProof (val_rel_litint_source with H) as "->" |
+         iPoseProof (val_rel_litbool_source with H) as "->" |
+         iPoseProof (val_rel_litfn_source with H) as "->" |
+         iPoseProof (val_rel_litunit_source with H) as "->" |
+         iPoseProof (val_rel_litpoison_source with H) as "->" |
+         idtac].
+Tactic Notation "val_discr_target" constr(H) :=
+  first [iPoseProof (val_rel_litint_target with H) as "->" |
+         iPoseProof (val_rel_litbool_target with H) as "->" |
+         iPoseProof (val_rel_litfn_target with H) as "->" |
+         iPoseProof (val_rel_litunit_target with H) as "->" |
+         iPoseProof (val_rel_litpoison_target with H) as "->" |
+         idtac].
+
+Lemma val_rel_func `{heapbijG Σ} v1 v2 v3 : val_rel v1 v2 -∗ val_rel v1 v3 -∗ ⌜v2 = v3⌝.
+Proof.
+  iIntros "Hv1 Hv2". iInduction v2 as [[n2 | b2 | | | l2 | f2 ] | v2_1 v2_2 | v2 | v2] "IH" forall (v1 v3); val_discr_source "Hv1"; val_discr_target "Hv2"; try done.
+  - iPoseProof (val_rel_loc_source with "Hv1") as (?) "(-> & Hl1)".
+    iPoseProof (val_rel_loc_target with "Hv2") as (?) "(-> & Hl2)".
+    by iPoseProof (heap_bij_loc_func with "Hl1 Hl2") as "->".
+  - iPoseProof (val_rel_pair_source with "Hv1") as (??) "(-> & Hv1_1 & Hv1_2)".
+    iPoseProof (val_rel_pair_target with "Hv2") as (??) "(-> & Hv2_1 & Hv2_2)".
+    iPoseProof ("IH" with "Hv1_1 Hv2_1") as "->".
+    by iPoseProof ("IH1" with "Hv1_2 Hv2_2") as "->".
+  - iPoseProof (val_rel_injl_source with "Hv1") as (?) "(-> & Hv1)".
+    iPoseProof (val_rel_injl_target with "Hv2") as (?) "(-> & Hv2)".
+    by iPoseProof ("IH" with "Hv1 Hv2") as "->".
+  - iPoseProof (val_rel_injr_source with "Hv1") as (?) "(-> & Hv1)".
+    iPoseProof (val_rel_injr_target with "Hv2") as (?) "(-> & Hv2)".
+    by iPoseProof ("IH" with "Hv1 Hv2") as "->".
+Qed.
+Lemma val_rel_inj `{heapbijG Σ} v1 v2 v3 : val_rel v2 v1 -∗ val_rel v3 v1 -∗ ⌜v2 = v3⌝.
+Proof.
+  iIntros "Hv1 Hv2". iInduction v2 as [[n2 | b2 | | | l2 | f2 ] | v2_1 v2_2 | v2 | v2] "IH" forall (v1 v3); val_discr_target "Hv1"; val_discr_source "Hv2"; try done.
+  - iPoseProof (val_rel_loc_target with "Hv1") as (?) "(-> & Hl1)".
+    iPoseProof (val_rel_loc_source with "Hv2") as (?) "(-> & Hl2)".
+    by iPoseProof (heap_bij_loc_inj with "Hl1 Hl2") as "->".
+  - iPoseProof (val_rel_pair_target with "Hv1") as (??) "(-> & Hv1_1 & Hv1_2)".
+    iPoseProof (val_rel_pair_source with "Hv2") as (??) "(-> & Hv2_1 & Hv2_2)".
+    iPoseProof ("IH" with "Hv1_1 Hv2_1") as "->".
+    by iPoseProof ("IH1" with "Hv1_2 Hv2_2") as "->".
+  - iPoseProof (val_rel_injl_target with "Hv1") as (?) "(-> & Hv1)".
+    iPoseProof (val_rel_injl_source with "Hv2") as (?) "(-> & Hv2)".
+    by iPoseProof ("IH" with "Hv1 Hv2") as "->".
+  - iPoseProof (val_rel_injr_target with "Hv1") as (?) "(-> & Hv1)".
+    iPoseProof (val_rel_injr_source with "Hv2") as (?) "(-> & Hv2)".
+    by iPoseProof ("IH" with "Hv1 Hv2") as "->".
+Qed.
+
+
+Section definitions.
+  Context `{heapbijG Σ}.
+
+  (** We require the [lock_state]s to be the same, pointwise *)
+  Definition alloc_rel b_t b_s P : iProp Σ :=
+    (∃ (n : option nat) vs_t vs_s,
+        ⌜length vs_t = default 0 n⌝ ∗
+      ([∗ list] i↦v_t;v_s∈vs_t;vs_s,
+          (∃ st q, ⌜P (Loc b_t i) (Loc b_s i) q⌝ ∗ val_rel v_t v_s ∗
+                    if q is Some q' then
+                      (Loc b_t i)↦t[st]{#q'} v_t ∗ (Loc b_s i)↦s[st]{#q'} v_s
+                    else
+                      True)) ∗
+      †Loc b_t 0 …?t n ∗
+      †Loc b_s 0 …?s n).
+
+  Lemma alloc_rel_mono (P' P : _ → _ → _ → Prop) b_t b_s:
+    (∀ q o, P (Loc b_t o) (Loc b_s o) q → P' (Loc b_t o) (Loc b_s o) q) →
+    alloc_rel b_t b_s P -∗
+    alloc_rel b_t b_s P'.
+  Proof.
+    iIntros (HP) "(%n&%vs_s&%vs_t&%&Hvs&?)".
+    iExists _, _, _. iFrame. iSplit; [done|].
+    iApply (big_sepL2_impl with "Hvs").
+    iIntros "!>" (?????) "(%st&%q&%&?&?)".
+    iExists _, q. iFrame. iPureIntro. by apply: HP.
+  Qed.
+
+  Lemma alloc_rel_read (b : bool) b_t b_s σ_s σ_t o v n (P : _ → _ → _ → Prop):
+    heap σ_s !! Loc b_s o = Some (RSt n, v) →
+    (∀ q, P (Loc b_t o) (Loc b_s o) q → ∃ q', q = Some q' ∧ if b then q' = 1%Qp else True) →
+    alloc_rel b_t b_s P -∗
+    heap_ctx sheapG_allocN_source (heap σ_s) (used_blocks σ_s) -∗
+    heap_ctx sheapG_allocN_target (heap σ_t) (used_blocks σ_t) -∗
+    ∃ n' v', ⌜heap σ_t !! Loc b_t o = Some (RSt n', v')⌝ ∗ ⌜if b then n' = n else True⌝ ∗ val_rel v' v.
+  Proof.
+    iIntros (? HP).
+    iDestruct 1 as (? vs_t vs_s Hlen) "(Hl_s & Halloc_t & Halloc_s)".
+    iIntros "Hσ_s Hσ_t".
+    iDestruct (big_sepL2_length with "Hl_s") as %?.
+
+    iDestruct (heap_freeable_lookup with "Hσ_s Halloc_s") as %[n' [? Hl]]; [done..|].
+    rewrite Loc_add in Hl. move: Hl => [] ?; simplify_eq/=.
+    have [v_s Hv_s]:= lookup_lt_is_Some_2 vs_s n' ltac:(lia).
+    have [v_t Hv_t]:= lookup_lt_is_Some_2 vs_t n' ltac:(lia).
+    iDestruct (big_sepL2_insert_acc with "Hl_s") as "[(%st''&%q'&%HP'&Hv&Hl_s) Hclose]"; [done..|].
+    have [?[??]] := HP _ HP'. subst.
+    iDestruct "Hl_s" as "[Hl_t Hl_s]".
+    case_match; subst.
+    - iDestruct (heap_read_st_1 with "Hσ_s Hl_s") as %Hl_s.
+      iDestruct (heap_read_st_1 with "Hσ_t Hl_t") as %Hl_t.
+      simplify_eq/=.
+      iExists _, _. by repeat (iSplitR; [done|]).
+    - iDestruct (heap_read_st with "Hσ_s Hl_s") as %[? Hl_s].
+      iDestruct (heap_read_st with "Hσ_t Hl_t") as %[? Hl_t].
+      destruct st''; simplify_eq/=.
+      iExists _, _. by repeat (iSplitR; [done|]).
+  Qed.
+
+  Lemma alloc_rel_write b_t b_s σ_s σ_t o v st st' v_s' v_t' (P : _ → _ → _ → Prop):
+    heap σ_s !! Loc b_s o = Some (st, v) →
+    (∀ q, P (Loc b_t o) (Loc b_s o) q → q = Some 1%Qp) →
+    alloc_rel b_t b_s P -∗
+    heap_ctx sheapG_allocN_source (heap σ_s) (used_blocks σ_s) -∗
+    heap_ctx sheapG_allocN_target (heap σ_t) (used_blocks σ_t) -∗
+    val_rel v_t' v_s' ==∗
+    alloc_rel b_t b_s P ∗
+    heap_ctx sheapG_allocN_source (<[Loc b_s o := (st', v_s')]> (heap σ_s)) (used_blocks σ_s) ∗
+    heap_ctx sheapG_allocN_target (<[Loc b_t o := (st', v_t')]> (heap σ_t)) (used_blocks σ_t).
+  Proof.
+    iIntros (? HP).
+    iDestruct 1 as (n vs_t vs_s Hlen) "(Hl_s & Halloc_t & Halloc_s)".
+    iIntros "Hσ_s Hσ_t Hval".
+    iDestruct (big_sepL2_length with "Hl_s") as %?.
+
+    iDestruct (heap_freeable_lookup with "Hσ_s Halloc_s") as %[n' [? Hl]]; [done..|].
+    rewrite Loc_add in Hl. move: Hl => [] ?; simplify_eq/=.
+    have [v_s Hv_s]:= lookup_lt_is_Some_2 vs_s n' ltac:(lia).
+    have [v_t Hv_t]:= lookup_lt_is_Some_2 vs_t n' ltac:(lia).
+    iDestruct (big_sepL2_insert_acc with "Hl_s") as "[(%st''&%q'&%HP'&Hv'&Hl_s) Hclose]"; [done..|].
+    have ? := HP _ HP'. subst.
+    iDestruct "Hl_s" as "[Hl_t Hl_s]".
+    iDestruct (heap_read_st_1 with "Hσ_s Hl_s") as %Hl_s.
+    iDestruct (heap_read_st_1 with "Hσ_t Hl_t") as %Hl_t.
+    simplify_eq/=.
+
+    iMod (heap_write with "Hσ_s Hl_s") as "[$ Hl_s]".
+    iMod (heap_write with "Hσ_t Hl_t") as "[$ Hl_t]".
+    iModIntro.
+    iExists _, _, _.
+    iFrame "Halloc_t Halloc_s".
+    iSplitR; last first.
+    - iApply "Hclose". iExists _, (Some _). by iFrame.
+    - iPureIntro. rewrite insert_length. lia.
+  Qed.
+
+  Lemma alloc_rel_P_holds (P : _ → _ → _ → Prop) b_t b_s σ_s o s:
+    heap σ_s !! Loc b_s o = Some s →
+    alloc_rel b_t b_s P -∗
+    heap_ctx sheapG_allocN_source (heap σ_s) (used_blocks σ_s) -∗
+    ⌜∃ q, P (Loc b_t o) (Loc b_s o) q⌝%Qp.
+  Proof.
+    iIntros (?).
+    iDestruct 1 as (? vs_t vs_s Hlen) "(Hl_s & Halloc_t & Halloc_s)".
+    iIntros "Hσ_s".
+    iDestruct (big_sepL2_length with "Hl_s") as %?.
+
+    iDestruct (heap_freeable_lookup with "Hσ_s Halloc_s") as %[n' [? Hl]]; [done..|].
+    rewrite Loc_add in Hl. move: Hl => [] ?; simplify_eq/=.
+    have [v_s Hv_s]:= lookup_lt_is_Some_2 vs_s n' ltac:(lia).
+    have [v_t Hv_t]:= lookup_lt_is_Some_2 vs_t n' ltac:(lia).
+    iDestruct (big_sepL2_insert_acc with "Hl_s") as "[(%st''&%q'&%HP'&Hl_s) _]"; [done..|].
+    iPureIntro. naive_solver.
+  Qed.
+
+  Lemma alloc_rel_remove_frac (P' P : _ → _ → _ → Prop) q1 q2 qd b_t b_s σ_s o v_s st:
+    heap σ_s !! Loc b_s o = Some (RSt st, v_s) →
+    (∀ q, P (Loc b_t o) (Loc b_s o) q → q = Some q1) →
+    P' (Loc b_t o) (Loc b_s o) q2 →
+    (∀ q o', o ≠ o' → P (Loc b_t o') (Loc b_s o') q → P' (Loc b_t o') (Loc b_s o') q) →
+    (if q2 is Some q2' then q1 = qd + q2' else q1 = qd)%Qp →
+    (q2 = None → st = 0) →
+    alloc_rel b_t b_s P -∗
+    heap_ctx sheapG_allocN_source (heap σ_s) (used_blocks σ_s)
+    ==∗
+    ∃ v_t,
+      (Loc b_t o)↦t{#qd}v_t ∗
+      (Loc b_s o)↦s{#qd}v_s ∗
+      val_rel v_t v_s ∗
+      alloc_rel b_t b_s P' ∗
+      heap_ctx sheapG_allocN_source (heap σ_s) (used_blocks σ_s).
+  Proof.
+    iIntros (? Hq1 Hq2 Hsame Hdiff Hst0).
+    iDestruct 1 as (n vs_t vs_s Hlen) "(Hvs & Halloc_t & Halloc_s)".
+    iIntros "Hσ_s".
+    iDestruct (big_sepL2_length with "Hvs") as %?.
+
+    iDestruct (heap_freeable_lookup with "Hσ_s Halloc_s") as %[n' [? Hl]]; [done..|].
+    rewrite Loc_add in Hl. move: Hl => [] ?; simplify_eq/=.
+    have [v_s' Hv_s]:= lookup_lt_is_Some_2 vs_s n' ltac:(lia).
+    have [v_t Hv_t]:= lookup_lt_is_Some_2 vs_t n' ltac:(lia).
+    have Hv_s':= take_drop_middle _ _ _ Hv_s.
+    have Hv_t':= take_drop_middle _ _ _ Hv_t.
+    rewrite -{1}Hv_s' -{1}Hv_t' big_sepL2_app_same_length /= ?take_length_le ?Nat.add_0_r; [|lia..].
+    iDestruct "Hvs" as "(Hvs_1&Hl&Hvs_2)".
+    iDestruct "Hl" as (st' q ?%Hq1) "[#Hv Hp]". subst.
+    iDestruct "Hp" as "[Hl_t Hl_s]".
+    iDestruct (heap_read_st with "Hσ_s Hl_s") as %[??]; destruct st' as [|n'']; simplify_eq/=.
+
+    destruct q2; subst.
+    - iDestruct (heap_mapsto_split _ _ _ _ 0 with "Hl_t") as "[Hl_t1 Hl_t2]"; [done..|].
+      iDestruct (heap_mapsto_split _ _ _ _ 0 with "Hl_s") as "[Hl_s1 Hl_s2]"; [done..|].
+      iModIntro.
+      iExists _. iFrame "∗Hv".
+      iExists _, vs_t, vs_s. iFrame. iSplit; [done|].
+      rewrite -{3}Hv_s' -{3}Hv_t' big_sepL2_app_same_length /= ?take_length_le ?Nat.add_0_r; [|lia..].
+      iSplitL "Hvs_1"; [|iSplitR "Hvs_2"].
+      + iApply (big_sepL2_impl with "Hvs_1").
+        iIntros "!>" (??? ?%take_lookup_Some ?%take_lookup_Some) "[%s [%q' [% Hp]]]".
+        iExists s, q'. iFrame. iPureIntro.
+        apply: Hsame; [lia| done].
+      + iExists _, _. iSplit; [done|]. by iFrame.
+      + iApply (big_sepL2_impl with "Hvs_2").
+        iIntros "!>" (??? ??) "[%s [%q' [% Hp]]]".
+        iExists s, q'. iFrame. iPureIntro.
+        apply: Hsame; [lia |done].
+    - have ->: n'' = 0 by naive_solver lia.
+      iModIntro.
+      iExists _. iFrame "∗Hv".
+      iExists _, vs_t, vs_s. iFrame. iSplit; [done|].
+      rewrite -{3}Hv_s' -{3}Hv_t' big_sepL2_app_same_length /= ?take_length_le ?Nat.add_0_r; [|lia..].
+      iSplitL "Hvs_1"; [|iSplitR "Hvs_2"].
+      + iApply (big_sepL2_impl with "Hvs_1").
+        iIntros "!>" (??? ?%take_lookup_Some ?%take_lookup_Some) "[%s [%q' [% Hp]]]".
+        iExists s, q'. iFrame. iPureIntro.
+        apply: Hsame; [lia|done].
+      + iExists _, _. iSplit; [done|] => /=. iFrame "Hv".
+      + iApply (big_sepL2_impl with "Hvs_2").
+        iIntros "!>" (??? ??) "[%s [%q' [% Hp]]]".
+        iExists s, q'. iFrame. iPureIntro.
+        apply: Hsame; [lia|done].
+        Unshelve.
+        apply: WSt.
+  Qed.
+
+  Lemma alloc_rel_add_frac (P' P : _ → _ → _ → Prop) q b_t b_s σ_s o v_s v_t:
+    (∀ q', P (Loc b_t o) (Loc b_s o) q' → P' (Loc b_t o) (Loc b_s o) (Some (if q' is Some q'' then (q + q'')%Qp else q))) →
+    (∀ q o', o ≠ o' → P (Loc b_t o') (Loc b_s o') q → P' (Loc b_t o') (Loc b_s o') q) →
+    alloc_rel b_t b_s P -∗
+    (Loc b_t o)↦t{#q}v_t -∗
+    (Loc b_s o)↦s{#q}v_s -∗
+    val_rel v_t v_s -∗
+    heap_ctx sheapG_allocN_source (heap σ_s) (used_blocks σ_s)
+    ==∗
+      alloc_rel b_t b_s P' ∗
+      heap_ctx sheapG_allocN_source (heap σ_s) (used_blocks σ_s).
+  Proof.
+    iIntros (Hq Hsame).
+    iDestruct 1 as (n vs_t vs_s Hlen) "(Hvs & Halloc_t & Halloc_s)".
+    iIntros "Hl_t Hl_s Hv Hσ_s".
+    iDestruct (big_sepL2_length with "Hvs") as %?.
+
+    iDestruct (heap_read with "Hσ_s Hl_s") as %[??].
+    iDestruct (heap_freeable_lookup with "Hσ_s Halloc_s") as %[n' [? Hl]]; [done..|].
+    rewrite Loc_add in Hl. move: Hl => [] ?; simplify_eq/=.
+    have [v_s' Hv_s]:= lookup_lt_is_Some_2 vs_s n' ltac:(lia).
+    have [v_t' Hv_t]:= lookup_lt_is_Some_2 vs_t n' ltac:(lia).
+    have Hv_s':= take_drop_middle _ _ _ Hv_s.
+    have Hv_t':= take_drop_middle _ _ _ Hv_t.
+    rewrite -{1}Hv_s' -{1}Hv_t' big_sepL2_app_same_length /= ?take_length_le ?Nat.add_0_r; [|lia..].
+    iDestruct "Hvs" as "(Hvs_1&Hl&Hvs_2)".
+    iDestruct "Hl" as (st' q' ?) "[Hv' Hp]". subst.
+
+    iModIntro. iFrame.
+    iExists n, (<[n' := v_t]>vs_t), (<[n' := v_s]>vs_s).
+    iSplit. { by rewrite insert_length. } iFrame.
+    rewrite !insert_take_drop; [|by apply: lookup_lt_Some..].
+    rewrite big_sepL2_app_same_length /= ?take_length_le ?Nat.add_0_r; [|lia..]. iFrame.
+    iSplitL "Hvs_1"; [|iSplitR "Hvs_2"].
+    - iApply (big_sepL2_impl with "Hvs_1").
+      iIntros "!>" (??? ?%take_lookup_Some ?%take_lookup_Some) "[%s [%q'' [% Hp]]]".
+      iExists s, q''. iFrame. iPureIntro.
+      apply: Hsame; [lia| done].
+    - iExists (if q' then st' else RSt 0), (Some (if q' is Some q'' then q + q'' else q))%Qp.
+      iSplit; first by eauto.
+      destruct q'; iFrame.
+      iDestruct "Hp" as "[Hp1 Hp2]".
+      iDestruct (heap_mapsto_agree with "[$Hp1 $Hl_t]") as %->.
+      iDestruct (heap_mapsto_agree with "[$Hp2 $Hl_s]") as %->.
+      iDestruct (heap_mapsto_combine_0 with "Hl_t Hp1") as "$".
+      iDestruct (heap_mapsto_combine_0 with "Hl_s Hp2") as "$".
+    - iApply (big_sepL2_impl with "Hvs_2").
+      iIntros "!>" (??? ??) "[%s [%q'' [% Hp]]]".
+      iExists s, q''. iFrame. iPureIntro.
+      apply: Hsame; [lia |done].
+  Qed.
+
+  Definition heap_bij_interp (L : gset (block * block)) (P : loc → loc → option Qp → Prop)  :=
+    (heap_bij_auth L ∗ [∗ set] p ∈ L, let '(b_t, b_s) := p in alloc_rel b_t b_s P)%I.
+End definitions.
+
+Section laws.
+  Context `{heapbijG Σ}.
+  Implicit Types (b_t b_s : block) (l_t l_s : loc).
+
+  Lemma heap_bij_access L P b_t b_s:
+    heap_bij_interp L P -∗
+    b_t ⇔h b_s -∗
+    ⌜(b_t, b_s) ∈ L⌝ ∗
+    alloc_rel b_t b_s P ∗
+    (∀ P' : _ → _ → _  → Prop,
+        ⌜∀ b_t' b_s' o q, b_t' ≠ b_t → b_s' ≠ b_s → P (Loc b_t' o) (Loc b_s' o) q →
+                           P' (Loc b_t' o) (Loc b_s' o) q⌝ -∗
+        (* ⌜∀ π col l_s w, cols' !! π = Some col → col !! l_s = Some w → loc_chunk l_s = b_s ∨ ∃ col' w', cols !! π = Some col' ∧ col' !! l_s = Some  w'⌝ -∗ *)
+        (* ⌜∀ b' o' q, b' ≠ b_s → alloc_rel_pred cols (Loc b' o') q → alloc_rel_pred cols' (Loc b' o') q⌝ -∗ *)
+        alloc_rel b_t b_s P' -∗ heap_bij_interp L P').
+  Proof.
+    iIntros "Hinv Hrel". iDestruct "Hinv" as "(Hauth & Hheap)".
+    iDestruct (gset_bij_elem_of with "Hauth Hrel") as %Hin.
+    iPoseProof (big_sepS_delete with "Hheap") as "[He Hheap]"; first done.
+    iDestruct (gset_bij_own_valid with "Hauth") as %[_ Hbij].
+    iFrame. iSplit; [done|].
+    iIntros (P' HP) "Halloc". iFrame.
+    iApply big_sepS_delete; first done. iFrame.
+    iApply (big_sepS_impl with "Hheap").
+    iIntros "!>" ([??] ?) "Halloc".
+    iApply (alloc_rel_mono with "Halloc") => ?? /=.
+    set_unfold. destruct H0 as [Hin2 Hneq].
+    have ?:= gset_bijective_eq_iff _ _ _ _ _ _ Hin Hin2.
+    apply: HP => b'; naive_solver.
+  Qed.
+
+  Lemma heap_bij_insertN L l_t l_s v_t v_s n (P : _ → _ → _ → Prop):
+    n > 0 →
+    length v_s = n →
+    length v_t = n →
+    (∀ o, (∀ b_s, (loc_chunk l_t, b_s) ∉ L) →
+          (∀ b_t, (b_t, loc_chunk l_s) ∉ L) → P (l_t +ₗ o) (l_s +ₗ o) (Some 1%Qp)) →
+    heap_bij_interp L P -∗
+    l_t ↦t∗ v_t -∗
+    l_s ↦s∗ v_s -∗
+    ([∗ list] vt;vs∈v_t;v_s, val_rel vt vs) -∗
+    †l_t …t n -∗
+    †l_s …s n ==∗
+    heap_bij_interp ({[(loc_chunk l_t, loc_chunk l_s)]} ∪ L) P ∗
+    l_t ↔h l_s.
+  Proof.
+    iIntros (Hn Hl_s Hl_t HP) "Hinv Ht Hs Hrel Ha_t Ha_s".
+    iDestruct (heap_freeable_idx with "Ha_t") as %?.
+    iDestruct (heap_freeable_idx with "Ha_s") as %?.
+    iDestruct "Hinv" as "(Hauth & Hheap)".
+    pose (b_t := loc_chunk l_t). pose (b_s := loc_chunk l_s).
+    iAssert ((¬ ⌜set_Exists (λ '(b_t', b_s'), b_t = b_t') L⌝)%I) as "%Hext_t".
+    { iIntros (([b_t' b_s'] & Hin & <-)).
+      iPoseProof (big_sepS_elem_of with "Hheap") as "Hr"; first by apply Hin.
+      iDestruct "Hr" as (n' v_t' v_s') "(_ & _ & Ha_t' & _)".
+      by iApply (heap_freeable_excl with "Ha_t Ha_t'").
+    }
+    iAssert ((¬ ⌜set_Exists (λ '(b_t', b_s'), b_s = b_s') L⌝)%I) as "%Hext_s".
+    { iIntros (([b_t' b_s'] & Hin & <-)).
+      iPoseProof (big_sepS_elem_of with "Hheap") as "Hr"; first by apply Hin.
+      iDestruct "Hr" as (n' v_t' v_s') "(_ & _ & _ & Ha_s')".
+      by iApply (heap_freeable_excl with "Ha_s Ha_s'").
+    }
+    iMod ((gset_bij_own_extend b_t b_s) with "Hauth") as "[Hinv #Helem]".
+    - intros b_s' Hb_s'. apply Hext_t. by exists (b_t, b_s').
+    - intros b_t' Hb_t'. apply Hext_s. by exists (b_t', b_s).
+    - iModIntro.
+      iSplitL; first last. { iSplitL; first done. iPureIntro; lia. }
+      iFrame. iApply big_sepS_insert. { contradict Hext_t. by exists (b_t, b_s). }
+      iFrame. iExists (Some n), v_t, v_s. iFrame.
+      destruct l_t, l_s; cbn in *; subst. iFrame.
+      iSplit; [done|].
+      iDestruct (big_sepL2_sepL_2 with "Ht Hs") as "Hvs"; [done|].
+      iCombine "Hrel" "Hvs" as "Hvs". rewrite -big_sepL2_sep.
+      iApply (big_sepL2_impl with "Hvs").
+      iIntros "!>" (?????) "(Hv&Ht&Hs)". iExists _, (Some 1%Qp). iFrame.
+      iPureIntro. apply HP => ??.
+      + apply: Hext_t. eexists _. naive_solver.
+      + apply: Hext_s. eexists _. naive_solver.
+  Qed.
+End laws.
